Skip to content
This repository

A modern list library for Emacs

Fetching latest commit…

Cannot retrieve the latest commit at this time

README.md

dash.el Build Status

A modern list api for Emacs. No 'cl required.

Installation

It's available on marmalade and Melpa:

M-x package-install dash

Or you can just dump dash.el in your load path somewhere.

Functions

There are also anaphoric versions of these functions where that makes sense, prefixed with two dashs instead of one.

Anaphoric functions

While -map takes a function to map over the list, you can also use the anaphoric form with double dashes - which will then be executed with it exposed as the list item. Here's an example:

(-map (lambda (n) (* n n)) '(1 2 3 4)) ;; normal version

(--map (* it it) '(1 2 3 4)) ;; anaphoric version

of course the original can also be written like

(defun square (n) (* n n))

(-map 'square '(1 2 3 4))

which demonstrates the usefulness of both versions.

Documentation and examples

-map (fn list)

Returns a new list consisting of the result of applying fn to the items in list.

(-map (lambda (num) (* num num)) '(1 2 3 4)) ;; => '(1 4 9 16)
(-map 'square '(1 2 3 4)) ;; => '(1 4 9 16)
(--map (* it it) '(1 2 3 4)) ;; => '(1 4 9 16)

-reduce-from (fn initial-value list)

Returns the result of applying fn to initial-value and the first item in list, then applying fn to that result and the 2nd item, etc. If list contains no items, returns initial-value and fn is not called.

In the anaphoric form --reduce-from, the accumulated value is exposed as acc.

(-reduce-from '+ 7 '(1 2)) ;; => 10
(-reduce-from (lambda (memo item) (+ memo item)) 7 '(1 2)) ;; => 10
(--reduce-from (+ acc it) 7 '(1 2 3)) ;; => 13

-reduce (fn list)

Returns the result of applying fn to the first 2 items in list, then applying fn to that result and the 3rd item, etc. If list contains no items, fn must accept no arguments as well, and reduce returns the result of calling fn with no arguments. If list has only 1 item, it is returned and fn is not called.

In the anaphoric form --reduce, the accumulated value is exposed as acc.

(-reduce '+ '(1 2)) ;; => 3
(-reduce (lambda (memo item) (format "%s-%s" memo item)) '(1 2 3)) ;; => "1-2-3"
(--reduce (format "%s-%s" acc it) '(1 2 3)) ;; => "1-2-3"

-filter (fn list)

Returns a new list of the items in list for which fn returns a non-nil value.

Alias: -select

(-filter (lambda (num) (= 0 (% num 2))) '(1 2 3 4)) ;; => '(2 4)
(-filter 'even? '(1 2 3 4)) ;; => '(2 4)
(--filter (= 0 (% it 2)) '(1 2 3 4)) ;; => '(2 4)

-remove (fn list)

Returns a new list of the items in list for which fn returns nil.

Alias: -reject

(-remove (lambda (num) (= 0 (% num 2))) '(1 2 3 4)) ;; => '(1 3)
(-remove 'even? '(1 2 3 4)) ;; => '(1 3)
(--remove (= 0 (% it 2)) '(1 2 3 4)) ;; => '(1 3)

-keep (fn list)

Returns a new list of the non-nil results of applying fn to the items in list.

(-keep 'cdr '((1 2 3) (4 5) (6))) ;; => '((2 3) (5))
(-keep (lambda (num) (when (> num 3) (* 10 num))) '(1 2 3 4 5 6)) ;; => '(40 50 60)
(--keep (when (> it 3) (* 10 it)) '(1 2 3 4 5 6)) ;; => '(40 50 60)

-flatten (l)

Takes a nested list l and returns its contents as a single, flat list.

(-flatten '((1))) ;; => '(1)
(-flatten '((1 (2 3) (((4 (5))))))) ;; => '(1 2 3 4 5)

-concat (&rest lists)

Returns a new list with the concatenation of the elements in the supplied lists.

(-concat '(1)) ;; => '(1)
(-concat '(1) '(2)) ;; => '(1 2)
(-concat '(1) '(2 3) '(4)) ;; => '(1 2 3 4)

-mapcat (fn list)

Returns the result of applying concat to the result of applying map to fn and list. Thus function fn should return a collection.

(-mapcat 'list '(1 2 3)) ;; => '(1 2 3)
(-mapcat (lambda (item) (list 0 item)) '(1 2 3)) ;; => '(0 1 0 2 0 3)
(--mapcat (list 0 it) '(1 2 3)) ;; => '(0 1 0 2 0 3)

-any? (fn list)

Returns t if (fn x) is non-nil for any x in list, else nil.

Alias: -some?

(-any? 'even? '(1 2 3)) ;; => t
(-any? 'even? '(1 3 5)) ;; => nil
(--any? (= 0 (% it 2)) '(1 2 3)) ;; => t

-all? (fn list)

Returns t if (fn x) is non-nil for all x in list, else nil.

Alias: -every?

(-all? 'even? '(1 2 3)) ;; => nil
(-all? 'even? '(2 4 6)) ;; => t
(--all? (= 0 (% it 2)) '(2 4 6)) ;; => t

-none? (fn list)

Returns t if (fn x) is nil for all x in list, else nil.

(-none? 'even? '(1 2 3)) ;; => nil
(-none? 'even? '(1 3 5)) ;; => t
(--none? (= 0 (% it 2)) '(1 2 3)) ;; => nil

-each (list fn)

Calls fn with every item in list. Returns nil, used for side-effects only.

(let (s) (-each '(1 2 3) (lambda (item) (setq s (cons item s))))) ;; => nil
(let (s) (-each '(1 2 3) (lambda (item) (setq s (cons item s)))) s) ;; => '(3 2 1)
(let (s) (--each '(1 2 3) (setq s (cons it s))) s) ;; => '(3 2 1)

-take (n list)

Returns a new list of the first n items in list, or all items if there are fewer than n.

(-take 3 '(1 2 3 4 5)) ;; => '(1 2 3)
(-take 17 '(1 2 3 4 5)) ;; => '(1 2 3 4 5)

-drop (n list)

Returns the tail of list without the first n items.

(-drop 3 '(1 2 3 4 5)) ;; => '(4 5)
(-drop 17 '(1 2 3 4 5)) ;; => '()

-take-while (fn list)

Returns a new list of successive items from list while (fn item) returns a non-nil value.

(-take-while 'even? '(1 2 3 4)) ;; => '()
(-take-while 'even? '(2 4 5 6)) ;; => '(2 4)
(--take-while (< it 4) '(1 2 3 4 3 2 1)) ;; => '(1 2 3)

-drop-while (fn list)

Returns the tail of list starting from the first item for which (fn item) returns nil.

(-drop-while 'even? '(1 2 3 4)) ;; => '(1 2 3 4)
(-drop-while 'even? '(2 4 5 6)) ;; => '(5 6)
(--drop-while (< it 4) '(1 2 3 4 3 2 1)) ;; => '(4 3 2 1)

-split-at (n list)

Returns a list of ((-take n list) (-drop n list))

(-split-at 3 '(1 2 3 4 5)) ;; => '((1 2 3) (4 5))
(-split-at 17 '(1 2 3 4 5)) ;; => '((1 2 3 4 5) nil)

-split-with (fn list)

Returns a list of ((-take-while fn list) (-drop-while fn list))

(-split-with 'even? '(1 2 3 4)) ;; => '(nil (1 2 3 4))
(-split-with 'even? '(2 4 5 6)) ;; => '((2 4) (5 6))
(--split-with (< it 4) '(1 2 3 4 3 2 1)) ;; => '((1 2 3) (4 3 2 1))

-interpose (sep list)

Returns a new list of all elements in list separated by sep.

(-interpose "-" '()) ;; => '()
(-interpose "-" '("a")) ;; => '("a")
(-interpose "-" '("a" "b" "c")) ;; => '("a" "-" "b" "-" "c")

-interleave (&rest lists)

Returns a new list of the first item in each list, then the second etc.

(-interleave '(1 2) '("a" "b")) ;; => '(1 "a" 2 "b")
(-interleave '(1 2) '("a" "b") '("A" "B")) ;; => '(1 "a" "A" 2 "b" "B")
(-interleave '(1 2 3) '("a" "b")) ;; => '(1 "a" 2 "b")

-replace-where (pred rep list)

Returns a new list where the elements in list that does not match the pred function are unchanged, and where the elements in list that do match the pred function are mapped through the rep function.

(-replace-where 'even? 'square '(1 2 3 4)) ;; => '(1 4 3 16)
(--replace-where (> it 2) (* it it) '(1 2 3 4)) ;; => '(1 2 9 16)
(--replace-where (= it 2) 17 '(1 2 3 4)) ;; => '(1 17 3 4)

-first (fn list)

Returns the first x in list where (fn x) is non-nil, else nil.

To get the first item in the list no questions asked, use car.

(-first 'even? '(1 2 3)) ;; => 2
(-first 'even? '(1 3 5)) ;; => nil
(--first (> it 2) '(1 2 3)) ;; => 3

-difference (list list2)

Return a new list with only the members of list that are not in list2. The test for equality is done with equal, or with -compare-fn if that's non-nil.

(-difference '() '()) ;; => '()
(-difference '(1 2 3) '(4 5 6)) ;; => '(1 2 3)
(-difference '(1 2 3 4) '(3 4 5 6)) ;; => '(1 2)

-intersection (list list2)

Return a new list containing only the elements that are members of both list and list2. The test for equality is done with equal, or with -compare-fn if that's non-nil.

(-intersection '() '()) ;; => '()
(-intersection '(1 2 3) '(4 5 6)) ;; => '()
(-intersection '(1 2 3 4) '(3 4 5 6)) ;; => '(3 4)

-distinct (list)

Return a new list with all duplicates removed. The test for equality is done with equal, or with -compare-fn if that's non-nil.

(-distinct '()) ;; => '()
(-distinct '(1 2 2 4)) ;; => '(1 2 4)

-contains? (list element)

Return whether list contains element. The test for equality is done with equal, or with -compare-fn if that's non-nil.

(-contains? '(1 2 3) 1) ;; => t
(-contains? '(1 2 3) 2) ;; => t
(-contains? '(1 2 3) 4) ;; => nil

-partial (fn &rest args)

Takes a function fn and fewer than the normal arguments to fn, and returns a fn that takes a variable number of additional args. When called, the returned function calls fn with args first and then additional args.

(funcall (-partial '- 5) 3) ;; => 2
(funcall (-partial '+ 5 2) 3) ;; => 10

-rpartial (fn &rest args)

Takes a function fn and fewer than the normal arguments to fn, and returns a fn that takes a variable number of additional args. When called, the returned function calls fn with the additional args first and then args.

Requires Emacs 24 or higher.

(funcall (-rpartial '- 5) 8) ;; => 3
(funcall (-rpartial '- 5 2) 10) ;; => 3

-> (x &optional form &rest more)

Threads the expr through the forms. Inserts x as the second item in the first form, making a list of it if it is not a list already. If there are more forms, inserts the first form as the second item in second form, etc.

(-> "Abc") ;; => "Abc"
(-> "Abc" (concat "def")) ;; => "Abcdef"
(-> "Abc" (concat "def") (concat "ghi")) ;; => "Abcdefghi"

->> (x form &rest more)

Threads the expr through the forms. Inserts x as the last item in the first form, making a list of it if it is not a list already. If there are more forms, inserts the first form as the last item in second form, etc.

(->> "Abc" (concat "def")) ;; => "defAbc"
(->> "Abc" (concat "def") (concat "ghi")) ;; => "ghidefAbc"
(->> 5 (- 8)) ;; => 3

--> (x form &rest more)

Threads the expr through the forms. Inserts x at the position signified by the token it in the first form. If there are more forms, inserts the first form at the position signified by it in in second form, etc.

(--> "def" (concat "abc" it "ghi")) ;; => "abcdefghi"
(--> "def" (concat "abc" it "ghi") (upcase it)) ;; => "ABCDEFGHI"
(--> "def" (concat "abc" it "ghi") upcase) ;; => "ABCDEFGHI"

Development

Run the tests with

./run-tests.sh

Create the docs with

./create-docs.sh

I highly recommend that you install these as a pre-commit hook, so that the tests are always running and the docs are always in sync:

cp pre-commit.sh .git/hooks/pre-commit

Oh, and don't edit README.md directly, it is auto-generated. Change readme-template.md or examples-to-docs.el instead.

License

Copyright (C) 2012 Magnar Sveen

Authors: Magnar Sveen magnars@gmail.com Keywords: lists

This program is free software; you can redistribute it and/or modify it under the terms of the GNU General Public License as published by the Free Software Foundation, either version 3 of the License, or (at your option) any later version.

This program is distributed in the hope that it will be useful, but WITHOUT ANY WARRANTY; without even the implied warranty of MERCHANTABILITY or FITNESS FOR A PARTICULAR PURPOSE. See the GNU General Public License for more details.

You should have received a copy of the GNU General Public License along with this program. If not, see http://www.gnu.org/licenses/.

Something went wrong with that request. Please try again.